Auto/Lib/BoolExtra.lean
@@ -1,9 +1,9 @@
 namespace Auto
 
-theorem Bool.beq_refl (a : Bool) : a == a := by
+theorem Bool.beq_refl {a : Bool} : a == a := by
   cases a <;> rfl
 
-theorem Bool.beq_eq (a b : Bool) (h : a == b) : a = b := by
+theorem Bool.eq_of_beq_eq_true {a b : Bool} (h : a == b) : a = b := by
   cases a <;> cases b <;> cases h <;> rfl
 
 theorem Bool.eq_false_of_ne_true {a : Bool} : a ≠ true → a = false := by
