Auto/Lib/ListExtra.lean
@@ -29,22 +29,24 @@ theorem List.ofFun_get?_eq_some (f : Nat → α) (n m : Nat) (h : n > m) :
       let h' := Nat.le_of_succ_le_succ h
       dsimp [ofFun, List.get?]; rw [IH (fun n => f (.succ n)) _ h']
 
+theorem List.beq_def [BEq α] {x y : List α} : (x == y) = x.beq y := rfl
+
 theorem List.beq_refl [BEq α] (H : ∀ (x : α), (x == x) = true) :
-  (l : List α) → (List.beq l l) = true
+  {l : List α} → (l == l) = true
 | .nil => rfl
 | .cons x xs => by
-  dsimp [List.beq]; rw [Bool.and_eq_true];
-  exact And.intro (H x) (List.beq_refl H xs)
+  rw [List.beq_def]; dsimp [List.beq]; rw [Bool.and_eq_true];
+  exact And.intro (H x) (List.beq_refl H)
 
-theorem List.beq_eq [BEq α] (H : ∀ (x y : α), (x == y) = true → x = y) :
-  (l₁ l₂ : List α) → List.beq l₁ l₂ → l₁ = l₂
+theorem List.eq_of_beq_eq_true [BEq α] (H : ∀ (x y : α), (x == y) = true → x = y) :
+  {l₁ l₂ : List α} → l₁ == l₂ → l₁ = l₂
 | .nil,       .nil       => fun _ => rfl
 | .nil,       .cons _ _  => fun h => by cases h
 | .cons _ _,  .nil       => fun h => by cases h
 | .cons u us, .cons v vs => fun h => by
-  dsimp [List.beq] at h; rw [Bool.and_eq_true] at h
+  rw [List.beq_def] at h; dsimp [List.beq] at h; rw [Bool.and_eq_true] at h
   have ⟨hHead, hTail⟩ := h
-  exact congr (congrArg _ (H _ _ hHead)) (List.beq_eq H _ _ hTail)
+  exact congr (congrArg _ (H _ _ hHead)) (List.eq_of_beq_eq_true H hTail)
 
 section
 
