Auto/Lib/OptionExtra.lean
@@ -18,4 +18,23 @@ theorem Option.allp_uniform (p : α → Prop) (x : Option α) :
   case none => exact True.intro
   case some v => apply h
 
+theorem Option.beq_none_none [BEq α] : (none (α:=α) == none) = true := rfl
+
+theorem Option.beq_none_some [BEq α] : (none (α:=α) == some x) = false := rfl
+
+theorem Option.beq_some_none [BEq α] : (some (α:=α) x == none) = false := rfl
+
+theorem Option.beq_some_some [BEq α] : (some (α:=α) x == some y) = (x == y) := rfl
+
+theorem Option.beq_refl [BEq α] (α_beq_refl : ∀ (x : α), x == x)
+  {x : Option α} : x == x := by
+  cases x
+  case none => rfl
+  case some => rw [beq_some_some]; rw [α_beq_refl]
+
+theorem Option.eq_of_beq_eq_true [BEq α] (α_eq_of_beq_eq_true : ∀ (x y : α), ((x == y) = true) → x = y)
+  {x y : Option α} (H : (x == y) = true) : x = y := by
+  cases x <;> cases y <;> try cases H <;> try rfl
+  rw [beq_some_some (α:=α)] at H; apply congrArg; apply α_eq_of_beq_eq_true _ _ H
+
 end Auto
